spot/GC.SPOT.HeapExpansion.fst
@@ -1131,10 +1131,43 @@ let spot_chunked_promote_object_head_split_preserves_chunked_alloc_shape
          res.fp_out <> 0UL /\
          GenInv.chunked_major_alloc_shape res.major_out res.fp_out fuel /\
          SpecMajorAlloc.major_fl_chain_terminates
-           res.major_out res.fp_out fuel = true))
+           res.major_out res.fp_out fuel = true /\
+         (let alloc_res =
+            SpecMajorAlloc.major_alloc_spec_with_fuel mh fp wosize fuel in
+          Seq.mem (fp <: obj_addr)
+            (MH.major_objects alloc_res.major_alloc_out) /\
+          Seq.mem (fp <: obj_addr) (MH.major_objects res.major_out))))
   =
   CheneyPreservation.chunked_promote_object_head_split_preserves_chunked_alloc_shape
     minor mh obj fp wosize fuel
+
+let spot_chunked_promote_object_head_split_preserves_remaining_head_wosize
+  (minor: minor_state) (mh: MH.major_heap) (obj: U64.t)
+  (fp: U64.t) (wosize: nat{wosize > 0}) (fuel: nat)
+  (remaining: nat)
+  : Lemma
+      (requires
+        fuel > 1 /\
+        fp <> 0UL /\
+        remaining > 0 /\
+        GenInv.chunked_major_alloc_shape mh fp fuel /\
+        SpecMajorAlloc.major_fl_chain_terminates mh fp fuel = true /\
+        SpecMajorAlloc.major_fl_head_wosize mh fp >=
+          wosize + 1 + remaining)
+      (ensures
+        (let res =
+           ChunkedPromote.chunked_promote_object_with_fuel
+             minor mh obj fp wosize fuel in
+         res.new_addr == fp /\
+         res.fp_out <> 0UL /\
+         GenInv.chunked_major_alloc_shape res.major_out res.fp_out fuel /\
+         SpecMajorAlloc.major_fl_chain_terminates
+           res.major_out res.fp_out fuel = true /\
+         SpecMajorAlloc.major_fl_head_wosize
+           res.major_out res.fp_out >= remaining))
+  =
+  CheneyPreservation.chunked_promote_object_head_split_preserves_remaining_head_wosize
+    minor mh obj fp wosize fuel remaining
 
 let spot_alloc_spec_head_split_alloc_wosize_single_chunk
   (major: heap) (fp: U64.t) (wosize: nat{wosize > 0})
